Prove that
\[
\log \left(\frac{x + 1}{x}\right)
  = 2\left\{\frac{1}{2x + 1} + \frac{1}{3(2x + 1)^{3}} + \frac{1}{5(2x + 1)^{5}} + \dots\right\}
\]
if $x > 0$, and that
\[
\log \frac{(x - 1)^{2}(x + 2)}{(x + 1)^{2}(x - 2)}
  = 2\left\{\frac{2}{x^{3} - 3x}
          + \frac{1}{3}\left(\frac{2}{x^{3} - 3x}\right)^{3}
          + \frac{1}{5}\left(\frac{2}{x^{3} - 3x}\right)^{5} + \dots\right\}
\]
if $x > 2$. Given that $\log 2 = .693\MS147\MS1\dots$ and $\log 3 = 1.098\MS612\MS3\dots$, show, by
putting $x = 10$ in the second formula, that $\log 11 = 2.397\MS895\dots$.
\MathTrip{1912.}

