The reader may verify that if $\alpha$,~$\beta$, $\gamma$,~$\delta$ are the roots of
\[
ax^{4} + 4bx^{3} + 6cx^{2} + 4dx + e = 0,
\]
then the equation whose roots are
\[
\tfrac{1}{12}a \{
  (\alpha - \beta)(\gamma - \delta) - (\gamma - \alpha)(\beta - \delta)
\},
\]
and two similar expressions formed by permuting $\alpha$,~$\beta$,~$\gamma$ cyclically, is
\[
4\theta^{3} - g_{2}\theta - g_{3} = 0,
\]
where
\[
g_{2} = ae - 4bd + 3c^{2},\quad
g_{3} = ace + 2bcd - ad^{2} - eb^{2} - c^{3}.
\]
It is clear that if two of $\alpha$,~$\beta$, $\gamma$,~$\delta$ are equal then two of the roots of this cubic
will be equal. Using the result of Ex.~8 we deduce that $g_{2}^{3} - 27g_{3}^{2} = 0$.

